Cleaned up name removal and chaining, fixed bug in pushenv back half

02Typed/Typechecking.thy
@@ -1,6 +1,6 @@
 theory Typechecking
   imports UnifiableType
-begin
+begin             
 
 subsection \<open>Typechecking\<close>
 
@@ -31,9 +31,10 @@ primrec typecheck' :: "subst \<Rightarrow> var set \<Rightarrow> 'a expr\<^sub>s
     in let (e\<^sub>u\<^sub>2, \<tau>\<^sub>2, vs\<^sub>2, \<kappa>\<^sub>2) = typecheck' \<Gamma> (insert v (vs \<union> vs\<^sub>1)) e\<^sub>2 
     in (App\<^sub>s e\<^sub>u\<^sub>1 e\<^sub>u\<^sub>2, Var v, insert v (vs\<^sub>1 \<union> vs\<^sub>2), \<kappa>\<^sub>1 @ \<kappa>\<^sub>2 @ [(\<tau>\<^sub>1, Arrow\<^sub>\<tau> \<tau>\<^sub>2 (Var v))]))"
 | "typecheck' \<Gamma> vs (Let\<^sub>s x e\<^sub>1 e\<^sub>2) = (
-    let (e\<^sub>u\<^sub>1, \<tau>\<^sub>1, vs\<^sub>1, \<kappa>\<^sub>1) = typecheck' \<Gamma> vs e\<^sub>1 
-    in let (e\<^sub>u\<^sub>2, \<tau>\<^sub>2, vs\<^sub>2, \<kappa>\<^sub>2) = typecheck' (\<Gamma>(x \<mapsto> \<tau>\<^sub>1)) (vs \<union> vs\<^sub>1) e\<^sub>2 
-    in (Let\<^sub>s x e\<^sub>u\<^sub>1 e\<^sub>u\<^sub>2, \<tau>\<^sub>2, vs\<^sub>1 \<union> vs\<^sub>2, \<kappa>\<^sub>1 @ \<kappa>\<^sub>2))"
+    let v = fresh vs
+    in let (e\<^sub>u\<^sub>1, \<tau>\<^sub>1, vs\<^sub>1, \<kappa>\<^sub>1) = typecheck' \<Gamma> (insert v vs) e\<^sub>1 
+    in let (e\<^sub>u\<^sub>2, \<tau>\<^sub>2, vs\<^sub>2, \<kappa>\<^sub>2) = typecheck' (\<Gamma>(x \<mapsto> Var v)) (insert v (vs \<union> vs\<^sub>1)) e\<^sub>2 
+    in (Let\<^sub>s x e\<^sub>u\<^sub>1 e\<^sub>u\<^sub>2, \<tau>\<^sub>2, insert v (vs\<^sub>1 \<union> vs\<^sub>2), \<kappa>\<^sub>1 @ \<kappa>\<^sub>2 @ [(Var v, \<tau>\<^sub>1)]))"
 
 text \<open>As with the unification algorithm, we create an induction method tailored to \<open>typecheck'\<close>.\<close>
 
@@ -53,12 +54,12 @@ lemma typecheck_induct [consumes 1, case_names Var\<^sub>sS Var\<^sub>sN Const\<
     P \<Gamma> (insert v (vs \<union> vs\<^sub>1)) e\<^sub>s\<^sub>2 e\<^sub>u\<^sub>2 \<tau>\<^sub>2 vs\<^sub>2 \<kappa>\<^sub>2 \<Longrightarrow>
     P \<Gamma> vs (App\<^sub>s e\<^sub>s\<^sub>1 e\<^sub>s\<^sub>2) (App\<^sub>s e\<^sub>u\<^sub>1 e\<^sub>u\<^sub>2) (Var v) (insert v (vs\<^sub>1 \<union> vs\<^sub>2)) 
       (\<kappa>\<^sub>1 @ \<kappa>\<^sub>2 @ [(\<tau>\<^sub>1, Arrow\<^sub>\<tau> \<tau>\<^sub>2 (Var v))])) \<Longrightarrow> 
-  (\<And>\<Gamma> vs e\<^sub>s\<^sub>1 e\<^sub>s\<^sub>2 x e\<^sub>u\<^sub>1 \<tau>\<^sub>1 vs\<^sub>1 \<kappa>\<^sub>1 e\<^sub>u\<^sub>2 \<tau>\<^sub>2 vs\<^sub>2 \<kappa>\<^sub>2. 
-    typecheck' \<Gamma> vs e\<^sub>s\<^sub>1 = (e\<^sub>u\<^sub>1, \<tau>\<^sub>1, vs\<^sub>1, \<kappa>\<^sub>1) \<Longrightarrow> 
-    typecheck' (\<Gamma>(x \<mapsto> \<tau>\<^sub>1)) (vs \<union> vs\<^sub>1) e\<^sub>s\<^sub>2 = (e\<^sub>u\<^sub>2, \<tau>\<^sub>2, vs\<^sub>2, \<kappa>\<^sub>2) \<Longrightarrow> 
-    P \<Gamma> vs e\<^sub>s\<^sub>1 e\<^sub>u\<^sub>1 \<tau>\<^sub>1 vs\<^sub>1 \<kappa>\<^sub>1 \<Longrightarrow> 
-    P (\<Gamma>(x \<mapsto> \<tau>\<^sub>1)) (vs \<union> vs\<^sub>1) e\<^sub>s\<^sub>2 e\<^sub>u\<^sub>2 \<tau>\<^sub>2 vs\<^sub>2 \<kappa>\<^sub>2 \<Longrightarrow>
-    P \<Gamma> vs (Let\<^sub>s x e\<^sub>s\<^sub>1 e\<^sub>s\<^sub>2) (Let\<^sub>s x e\<^sub>u\<^sub>1 e\<^sub>u\<^sub>2) \<tau>\<^sub>2 (vs\<^sub>1 \<union> vs\<^sub>2) (\<kappa>\<^sub>1 @ \<kappa>\<^sub>2)) \<Longrightarrow> 
+  (\<And>\<Gamma> vs e\<^sub>s\<^sub>1 e\<^sub>s\<^sub>2 x v e\<^sub>u\<^sub>1 \<tau>\<^sub>1 vs\<^sub>1 \<kappa>\<^sub>1 e\<^sub>u\<^sub>2 \<tau>\<^sub>2 vs\<^sub>2 \<kappa>\<^sub>2. v = fresh vs \<Longrightarrow> 
+    typecheck' \<Gamma> (insert v vs) e\<^sub>s\<^sub>1 = (e\<^sub>u\<^sub>1, \<tau>\<^sub>1, vs\<^sub>1, \<kappa>\<^sub>1) \<Longrightarrow> 
+    typecheck' (\<Gamma>(x \<mapsto> Var v)) (insert v (vs \<union> vs\<^sub>1)) e\<^sub>s\<^sub>2 = (e\<^sub>u\<^sub>2, \<tau>\<^sub>2, vs\<^sub>2, \<kappa>\<^sub>2) \<Longrightarrow> 
+    P \<Gamma> (insert v vs) e\<^sub>s\<^sub>1 e\<^sub>u\<^sub>1 \<tau>\<^sub>1 vs\<^sub>1 \<kappa>\<^sub>1 \<Longrightarrow> 
+    P (\<Gamma>(x \<mapsto> Var v)) (insert v (vs \<union> vs\<^sub>1)) e\<^sub>s\<^sub>2 e\<^sub>u\<^sub>2 \<tau>\<^sub>2 vs\<^sub>2 \<kappa>\<^sub>2 \<Longrightarrow>
+    P \<Gamma> vs (Let\<^sub>s x e\<^sub>s\<^sub>1 e\<^sub>s\<^sub>2) (Let\<^sub>s x e\<^sub>u\<^sub>1 e\<^sub>u\<^sub>2) \<tau>\<^sub>2 (insert v (vs\<^sub>1 \<union> vs\<^sub>2)) (\<kappa>\<^sub>1 @ \<kappa>\<^sub>2 @ [(Var v, \<tau>\<^sub>1)])) \<Longrightarrow> 
   P \<Gamma> vs e\<^sub>s e\<^sub>u \<tau> vs' \<kappa>"
   by (induction e\<^sub>s arbitrary: \<Gamma> vs e\<^sub>u \<tau> vs' \<kappa>) 
      (auto simp add: Let_def split: option.splits prod.splits)
@@ -70,13 +71,34 @@ lemma typecheck_to_valid_type [elim]: "typecheck' \<Gamma> vs e\<^sub>s = (e\<^s
 lemma typecheck_to_valid_expr [elim]: "typecheck' \<Gamma> vs e\<^sub>s = (e\<^sub>u, \<tau>, vs', \<kappa>) \<Longrightarrow> 
     valid_ty_subst \<Gamma> \<Longrightarrow> valid_ty_expr e\<^sub>u"
 proof (induction rule: typecheck_induct) 
-  case (Let\<^sub>s \<Gamma> vs e\<^sub>s\<^sub>1 e\<^sub>s\<^sub>2 x e\<^sub>u\<^sub>1 \<tau>\<^sub>1 vs\<^sub>1 \<kappa>\<^sub>1 e\<^sub>u\<^sub>2 \<tau>\<^sub>2 vs\<^sub>2 \<kappa>\<^sub>2)
+  case (Let\<^sub>s \<Gamma> vs e\<^sub>s\<^sub>1 e\<^sub>s\<^sub>2 x v e\<^sub>u\<^sub>1 \<tau>\<^sub>1 vs\<^sub>1 \<kappa>\<^sub>1 e\<^sub>u\<^sub>2 \<tau>\<^sub>2 vs\<^sub>2 \<kappa>\<^sub>2)
   moreover hence "valid_ty_term \<tau>\<^sub>1" by auto
   ultimately show ?case by simp
 qed simp_all
 
 lemma typecheck_erase [simp]: "typecheck' \<Gamma> vs e\<^sub>s = (e\<^sub>u, \<tau>, vs', \<kappa>) \<Longrightarrow> erase e\<^sub>u = e\<^sub>s"
   by (induction rule: typecheck_induct) simp_all
+
+lemma typecheck_finite [simp]: "typecheck' \<Gamma> vs e\<^sub>s = (e\<^sub>u, \<tau>, vs', \<kappa>) \<Longrightarrow> finite vs \<Longrightarrow> finite vs'"
+  by (induction rule: typecheck_induct) simp_all
+
+lemma typecheck_vars_distinct [simp]: "typecheck' \<Gamma> vs e\<^sub>s = (e\<^sub>u, \<tau>, vs', \<kappa>) \<Longrightarrow> finite vs \<Longrightarrow> 
+    vs \<inter> vs' = {}"
+  by (induction rule: typecheck_induct) auto
+
+lemma typecheck_type_vars [simp]: "typecheck' \<Gamma> vs e\<^sub>s = (e\<^sub>u, \<tau>, vs', \<kappa>) \<Longrightarrow> finite vs \<Longrightarrow> 
+    uvars \<tau> \<subseteq> vs' \<union> subst_vars \<Gamma>"
+  by (induction rule: typecheck_induct) auto
+
+lemma typecheck_type_in_old_vars [simp]: "typecheck' \<Gamma> vs e\<^sub>s = (e\<^sub>u, \<tau>, vs', \<kappa>) \<Longrightarrow> x \<in> vs \<Longrightarrow> 
+  finite vs \<Longrightarrow> x \<notin> subst_vars \<Gamma> \<Longrightarrow> x \<notin> uvars \<tau>"
+proof -
+  assume T: "typecheck' \<Gamma> vs e\<^sub>s = (e\<^sub>u, \<tau>, vs', \<kappa>)" and F: "finite vs"
+  hence "uvars \<tau> \<subseteq> vs' \<union> subst_vars \<Gamma>" by simp
+  moreover from T F have "vs \<inter> vs' = {}" by simp
+  moreover assume "x \<in> vs" and "x \<notin> subst_vars \<Gamma>" 
+  ultimately show "x \<notin> uvars \<tau>" by auto
+qed
 
 text \<open>Full typechecking is now easy. We generate our annotated expression, type term, and 
 constraints and then try to unify the constraint; if it fails, we fail, and if it succeeds, we 
@@ -106,13 +128,15 @@ indicated, and erases to the original expression. We prove it first for \<open>t
 full typechecker.\<close>
 
 lemma typecheck_success' [simp]: "typecheck' \<Gamma> vs e\<^sub>s = (e\<^sub>u, \<tau>, vs', \<kappa>) \<Longrightarrow> valid_ty_subst \<Gamma> \<Longrightarrow> 
-  unify \<kappa> = Some \<sigma>' \<Longrightarrow> \<sigma> specializes \<sigma>' \<Longrightarrow>
+  unify \<kappa> = Some \<sigma>' \<Longrightarrow> \<sigma> specializes \<sigma>' \<Longrightarrow> finite vs \<Longrightarrow> subst_vars \<Gamma> \<subseteq> vs \<Longrightarrow>
   map_option (to_type \<circ> subst \<sigma>) \<circ> \<Gamma> \<turnstile>\<^sub>t map_expr\<^sub>s to_type (map_expr\<^sub>s (subst \<sigma>) e\<^sub>u) : 
     to_type (subst \<sigma> \<tau>)"
 proof (induction arbitrary: \<sigma>' rule: typecheck_induct)
   case (Lam\<^sub>s \<Gamma> vs x u e\<^sub>s v e\<^sub>u \<tau> vs' \<kappa>)
-  hence "valid_ty_subst (\<Gamma>(x \<mapsto> Var v))" by simp
-  with Lam\<^sub>s have "map_option (to_type \<circ> subst \<sigma>) \<circ> \<Gamma>(x \<mapsto> Var v) \<turnstile>\<^sub>t 
+  moreover hence "valid_ty_subst (\<Gamma>(x \<mapsto> Var v))" by simp
+  moreover from Lam\<^sub>s have "subst_vars (\<Gamma>(x := None)) \<subseteq> vs" by simp
+  moreover hence "subst_vars (\<Gamma>(x \<mapsto> Var v)) \<subseteq> insert v vs" by auto
+  ultimately have "map_option (to_type \<circ> subst \<sigma>) \<circ> \<Gamma>(x \<mapsto> Var v) \<turnstile>\<^sub>t 
     map_expr\<^sub>s to_type (map_expr\<^sub>s (subst \<sigma>) e\<^sub>u) : to_type (subst \<sigma> \<tau>)" by blast
   hence "map_option (to_type \<circ> subst \<sigma>) \<circ> \<Gamma> \<turnstile>\<^sub>t 
     map_expr\<^sub>s to_type (map_expr\<^sub>s (subst \<sigma>) (Lam\<^sub>s x (Var v) e\<^sub>u)) : 
@@ -127,31 +151,38 @@ next
     map_expr\<^sub>s to_type (map_expr\<^sub>s (subst \<sigma>) e\<^sub>u\<^sub>1) : to_type (subst \<sigma> \<tau>\<^sub>1)" by blast
   from App\<^sub>s have "\<sigma>' unifies\<^sub>\<kappa> (\<kappa>\<^sub>1 @ \<kappa>\<^sub>2 @ [(\<tau>\<^sub>1, Arrow\<^sub>\<tau> \<tau>\<^sub>2 (Var v))])" by (metis unify_some) 
   hence "\<sigma>' unifies \<tau>\<^sub>1 and Arrow\<^sub>\<tau> \<tau>\<^sub>2 (Var v)" by simp
-  with App\<^sub>s have X: "\<sigma> unifies \<tau>\<^sub>1 and Arrow\<^sub>\<tau> \<tau>\<^sub>2 (Var v)" by fastforce
+  with App\<^sub>s have X: "\<sigma> unifies \<tau>\<^sub>1 and Arrow\<^sub>\<tau> \<tau>\<^sub>2 (Var v)" by fast
   from S2 obtain s\<^sub>4 where S4: "unify \<kappa>\<^sub>2 = Some s\<^sub>4 \<and> \<sigma>\<^sub>2 specializes s\<^sub>4" 
     using unify_append_snd by blast
-  with App\<^sub>s S2 have "\<sigma> specializes s\<^sub>4" by auto
-  with App\<^sub>s S4 have "map_option (to_type \<circ> subst \<sigma>) \<circ> \<Gamma> \<turnstile>\<^sub>t 
+  with App\<^sub>s S2 have Y: "\<sigma> specializes s\<^sub>4" by auto
+  from App\<^sub>s have "finite (insert v (vs \<union> vs\<^sub>1))" by simp
+  with App\<^sub>s S4 Y have "map_option (to_type \<circ> subst \<sigma>) \<circ> \<Gamma> \<turnstile>\<^sub>t 
     map_expr\<^sub>s to_type (map_expr\<^sub>s (subst \<sigma>) e\<^sub>u\<^sub>2) : to_type (subst \<sigma> \<tau>\<^sub>2)" by blast
   with T X have "map_option (to_type \<circ> subst \<sigma>) \<circ> \<Gamma> \<turnstile>\<^sub>t 
     map_expr\<^sub>s to_type (map_expr\<^sub>s (subst \<sigma>) (App\<^sub>s e\<^sub>u\<^sub>1 e\<^sub>u\<^sub>2)) : to_type (subst \<sigma> (Var v))" by simp
   thus ?case by blast
 next
-  case (Let\<^sub>s \<Gamma> vs e\<^sub>s\<^sub>1 e\<^sub>s\<^sub>2 x e\<^sub>u\<^sub>1 \<tau>\<^sub>1 vs\<^sub>1 \<kappa>\<^sub>1 e\<^sub>u\<^sub>2 \<tau>\<^sub>2 vs\<^sub>2 \<kappa>\<^sub>2)
+  case (Let\<^sub>s \<Gamma> vs e\<^sub>s\<^sub>1 e\<^sub>s\<^sub>2 x v e\<^sub>u\<^sub>1 \<tau>\<^sub>1 vs\<^sub>1 \<kappa>\<^sub>1 e\<^sub>u\<^sub>2 \<tau>\<^sub>2 vs\<^sub>2 \<kappa>\<^sub>2)
   moreover then obtain \<sigma>\<^sub>1 where "unify \<kappa>\<^sub>1 = Some \<sigma>\<^sub>1 \<and> \<sigma>' specializes \<sigma>\<^sub>1" by fastforce
   moreover with Let\<^sub>s have "\<sigma> specializes \<sigma>\<^sub>1" by auto
   ultimately have X: "map_option (to_type \<circ> subst \<sigma>) \<circ> \<Gamma> \<turnstile>\<^sub>t 
     map_expr\<^sub>s to_type (map_expr\<^sub>s (subst \<sigma>) e\<^sub>u\<^sub>1) : to_type (subst \<sigma> \<tau>\<^sub>1)" by blast
-  from Let\<^sub>s obtain s\<^sub>2 where S2: "unify \<kappa>\<^sub>2 = Some s\<^sub>2 \<and> \<sigma>' specializes s\<^sub>2" 
+  from Let\<^sub>s obtain \<sigma>\<^sub>2 where S2: "unify (\<kappa>\<^sub>2 @ [(Var v, \<tau>\<^sub>1)]) = Some \<sigma>\<^sub>2 \<and> \<sigma>' specializes \<sigma>\<^sub>2" 
     using unify_append_snd by blast
-  with Let\<^sub>s have Y: "\<sigma> specializes s\<^sub>2" by auto
-  from Let\<^sub>s have "valid_ty_term \<tau>\<^sub>1" by auto
-  with Let\<^sub>s have "valid_ty_subst (\<Gamma>(x \<mapsto> \<tau>\<^sub>1))" by simp
-  with Let\<^sub>s S2 Y have "map_option (to_type \<circ> subst \<sigma>) \<circ> \<Gamma>(x \<mapsto> \<tau>\<^sub>1) \<turnstile>\<^sub>t 
+  then obtain \<sigma>\<^sub>3 where S3: "unify \<kappa>\<^sub>2 = Some \<sigma>\<^sub>3 \<and> \<sigma>\<^sub>2 specializes \<sigma>\<^sub>3" by fastforce
+  with Let\<^sub>s S2 have Y: "\<sigma> specializes \<sigma>\<^sub>3" by auto
+  from Let\<^sub>s have Z: "valid_ty_subst (\<Gamma>(x \<mapsto> Var v))" by simp
+  from Let\<^sub>s have W: "finite (insert v (vs \<union> vs\<^sub>1))" by simp
+  from Let\<^sub>s have "subst_vars (\<Gamma>(x \<mapsto> Var v)) \<subseteq> insert v (vs \<union> vs\<^sub>1)" by auto
+  with Let\<^sub>s S3 Y Z W have A: "map_option (to_type \<circ> subst \<sigma>) \<circ> \<Gamma>(x \<mapsto> Var v) \<turnstile>\<^sub>t 
     map_expr\<^sub>s to_type (map_expr\<^sub>s (subst \<sigma>) e\<^sub>u\<^sub>2) : to_type (subst \<sigma> \<tau>\<^sub>2)" by blast
-  hence "(map_option (to_type \<circ> subst \<sigma>) \<circ> \<Gamma>)(x \<mapsto> to_type (subst \<sigma> \<tau>\<^sub>1)) \<turnstile>\<^sub>t 
-    map_expr\<^sub>s to_type (map_expr\<^sub>s (subst \<sigma>) e\<^sub>u\<^sub>2) : to_type (subst \<sigma> \<tau>\<^sub>2)" by simp
-  with X have "map_option (to_type \<circ> subst \<sigma>) \<circ> \<Gamma> \<turnstile>\<^sub>t 
+  from S2 obtain \<sigma>\<^sub>4 where S4: "unify [(Var v, \<tau>\<^sub>1)] = Some \<sigma>\<^sub>4 \<and> \<sigma>\<^sub>2 specializes \<sigma>\<^sub>4" 
+    using unify_append_snd by blast
+  from Let\<^sub>s have "v \<notin> subst_vars \<Gamma>" by auto
+  with Let\<^sub>s have "v \<notin> uvars \<tau>\<^sub>1" by simp
+  with S4 have "\<sigma>\<^sub>4 unifies Var v and \<tau>\<^sub>1" by (auto split: if_splits)
+  with Let\<^sub>s S2 S4 have "\<sigma> unifies Var v and \<tau>\<^sub>1" by fastforce
+  with X A have "map_option (to_type \<circ> subst \<sigma>) \<circ> \<Gamma> \<turnstile>\<^sub>t 
     map_expr\<^sub>s to_type (map_expr\<^sub>s (subst \<sigma>) (Let\<^sub>s x e\<^sub>u\<^sub>1 e\<^sub>u\<^sub>2)) : to_type (subst \<sigma> \<tau>\<^sub>2)" by simp
   thus ?case by blast
 qed simp_all
@@ -162,10 +193,10 @@ proof
   assume "typecheck e\<^sub>s = Some (e\<^sub>t, t)"
   then obtain e\<^sub>u \<tau> vs \<kappa> \<sigma> where T: "typecheck' Map.empty {} e\<^sub>s = (e\<^sub>u, \<tau>, vs, \<kappa>) \<and>
     unify \<kappa> = Some \<sigma> \<and> e\<^sub>t = map_expr\<^sub>s to_type (map_expr\<^sub>s (subst \<sigma>) e\<^sub>u) \<and> t = to_type (subst \<sigma> \<tau>)" 
-      by (auto split: option.splits prod.splits)
+    by (auto split: option.splits prod.splits)
   moreover hence "map_option (to_type \<circ> subst \<sigma>) \<circ> Map.empty \<turnstile>\<^sub>t 
     map_expr\<^sub>s to_type (map_expr\<^sub>s (subst \<sigma>) e\<^sub>u) : to_type (subst \<sigma> \<tau>)" 
-      by (metis typecheck_success' valid_empty_subst specializes_refl)
+      using typecheck_success' by fastforce
   moreover from T have "valid_ty_term \<tau>" and "valid_ty_expr e\<^sub>u" by auto
   ultimately show "Map.empty \<turnstile>\<^sub>t e\<^sub>t : t" by simp
   from T have "erase e\<^sub>u = e\<^sub>s" by (metis typecheck_erase)
@@ -183,27 +214,6 @@ rendered false by accepting too few expressions: we must prove that every single
 genuine failure, and the process of doing so essentially amounts to proving the correctness of the 
 whole algorithm. For this reason, although it may not appear so at first glance, the failure theorem 
 is the more important of the two.\<close>
-
-lemma typecheck_finite [simp]: "typecheck' \<Gamma> vs e\<^sub>s = (e\<^sub>u, \<tau>, vs', \<kappa>) \<Longrightarrow> finite vs \<Longrightarrow> finite vs'"
-  by (induction rule: typecheck_induct) simp_all
-
-lemma typecheck_vars_distinct [simp]: "typecheck' \<Gamma> vs e\<^sub>s = (e\<^sub>u, \<tau>, vs', \<kappa>) \<Longrightarrow> finite vs \<Longrightarrow> 
-    vs \<inter> vs' = {}"
-  by (induction rule: typecheck_induct) auto
-
-lemma typecheck_type_vars [simp]: "typecheck' \<Gamma> vs e\<^sub>s = (e\<^sub>u, \<tau>, vs', \<kappa>) \<Longrightarrow> finite vs \<Longrightarrow> 
-    uvars \<tau> \<subseteq> vs' \<union> subst_vars \<Gamma>"
-  by (induction rule: typecheck_induct) auto
-
-lemma typecheck_type_in_old_vars [simp]: "typecheck' \<Gamma> vs e\<^sub>s = (e\<^sub>u, \<tau>, vs', \<kappa>) \<Longrightarrow> x \<in> vs \<Longrightarrow> 
-  finite vs \<Longrightarrow> x \<notin> subst_vars \<Gamma> \<Longrightarrow> x \<notin> uvars \<tau>"
-proof -
-  assume T: "typecheck' \<Gamma> vs e\<^sub>s = (e\<^sub>u, \<tau>, vs', \<kappa>)" and F: "finite vs"
-  hence "uvars \<tau> \<subseteq> vs' \<union> subst_vars \<Gamma>" by simp
-  moreover from T F have "vs \<inter> vs' = {}" by simp
-  moreover assume "x \<in> vs" and "x \<notin> subst_vars \<Gamma>" 
-  ultimately show "x \<notin> uvars \<tau>" by auto
-qed
 
 lemma typecheck_expr_vars [simp]: "typecheck' \<Gamma> vs e\<^sub>s = (e\<^sub>u, \<tau>, vs', \<kappa>) \<Longrightarrow> finite vs \<Longrightarrow> 
     tyvars\<^sub>s e\<^sub>u \<subseteq> vs'"
@@ -229,11 +239,11 @@ proof (induction rule: typecheck_induct)
     uvars \<tau>\<^sub>2 \<subseteq> insert v (vs\<^sub>1 \<union> vs\<^sub>2 \<union> subst_vars \<Gamma>)" by auto
   with App\<^sub>s show ?case by auto
 next
-  case (Let\<^sub>s \<Gamma> vs e\<^sub>s\<^sub>1 e\<^sub>s\<^sub>2 x e\<^sub>u\<^sub>1 \<tau>\<^sub>1 vs\<^sub>1 \<kappa>\<^sub>1 e\<^sub>u\<^sub>2 \<tau>\<^sub>2 vs\<^sub>2 \<kappa>\<^sub>2)
+  case (Let\<^sub>s \<Gamma> vs e\<^sub>s\<^sub>1 e\<^sub>s\<^sub>2 x v e\<^sub>u\<^sub>1 \<tau>\<^sub>1 vs\<^sub>1 \<kappa>\<^sub>1 e\<^sub>u\<^sub>2 \<tau>\<^sub>2 vs\<^sub>2 \<kappa>\<^sub>2)
   moreover hence "finite vs\<^sub>1" by simp
-  ultimately have "constr_vars \<kappa>\<^sub>2 \<subseteq> vs\<^sub>2 \<union> subst_vars (\<Gamma>(x \<mapsto> \<tau>\<^sub>1))" by simp
-  moreover from Let\<^sub>s have "uvars \<tau>\<^sub>1 \<subseteq> vs\<^sub>1 \<union> subst_vars \<Gamma>" by simp
-  ultimately have "constr_vars \<kappa>\<^sub>2 \<subseteq> vs\<^sub>1 \<union> vs\<^sub>2 \<union> subst_vars \<Gamma>" by auto
+  ultimately have "constr_vars \<kappa>\<^sub>2 \<subseteq> vs\<^sub>2 \<union> subst_vars (\<Gamma>(x \<mapsto> Var v))" by simp
+  from Let\<^sub>s have "uvars \<tau>\<^sub>1 \<subseteq> vs\<^sub>1 \<union> subst_vars \<Gamma>" by simp
+  hence "uvars \<tau>\<^sub>1 \<subseteq> insert v (vs\<^sub>1 \<union> vs\<^sub>2 \<union> subst_vars \<Gamma>)" by auto
   with Let\<^sub>s show ?case by auto
 qed auto
 
@@ -327,70 +337,43 @@ next
   thus ?case by blast
 next
   case (Let\<^sub>s z e\<^sub>s\<^sub>1 e\<^sub>s\<^sub>2)
-  obtain e\<^sub>u\<^sub>1 \<tau>\<^sub>1 vs\<^sub>1 \<kappa>\<^sub>1 where T1: "typecheck' (\<Gamma>(x \<mapsto> Var y)) vs e\<^sub>s\<^sub>1 = (e\<^sub>u\<^sub>1, \<tau>\<^sub>1, vs\<^sub>1, \<kappa>\<^sub>1)" 
+  let ?v = "fresh vs"
+  obtain e\<^sub>u\<^sub>1 \<tau>\<^sub>1 vs\<^sub>1 \<kappa>\<^sub>1 where T1: "typecheck' (\<Gamma>(x \<mapsto> Var y)) (insert ?v vs) e\<^sub>s\<^sub>1 = (e\<^sub>u\<^sub>1, \<tau>\<^sub>1, vs\<^sub>1, \<kappa>\<^sub>1)"
     by (metis prod_cases4)
-  with Let\<^sub>s have TC1: "typecheck' (\<Gamma>(x \<mapsto> \<tau>')) vs e\<^sub>s\<^sub>1 =
+  with Let\<^sub>s have T1': "typecheck' (\<Gamma>(x \<mapsto> \<tau>')) (insert ?v vs) e\<^sub>s\<^sub>1 =
     (map_expr\<^sub>s (subst [y \<mapsto> \<tau>']) e\<^sub>u\<^sub>1, subst [y \<mapsto> \<tau>'] \<tau>\<^sub>1, vs\<^sub>1, constr_subst y \<tau>' \<kappa>\<^sub>1)" by blast
-  obtain e\<^sub>u\<^sub>2 \<tau>\<^sub>2 vs\<^sub>2 \<kappa>\<^sub>2 where T2: "typecheck' (\<Gamma>(x \<mapsto> Var y, z \<mapsto> \<tau>\<^sub>1)) (vs \<union> vs\<^sub>1) e\<^sub>s\<^sub>2 = 
+  obtain e\<^sub>u\<^sub>2 \<tau>\<^sub>2 vs\<^sub>2 \<kappa>\<^sub>2 where T2: "typecheck' (\<Gamma>(x \<mapsto> Var y, z \<mapsto> Var ?v)) (insert ?v (vs \<union> vs\<^sub>1)) e\<^sub>s\<^sub>2 =
     (e\<^sub>u\<^sub>2, \<tau>\<^sub>2, vs\<^sub>2, \<kappa>\<^sub>2)" by (metis prod_cases4)
-  show ?case
+  from Let\<^sub>s have "typecheck' (\<Gamma>(x \<mapsto> Var y)) vs (Let\<^sub>s z e\<^sub>s\<^sub>1 e\<^sub>s\<^sub>2) = (e\<^sub>u, \<tau>, vs', \<kappa>)" by blast
+  with T1 T2 have E: "e\<^sub>u = Let\<^sub>s z e\<^sub>u\<^sub>1 e\<^sub>u\<^sub>2 \<and> \<tau> = \<tau>\<^sub>2 \<and> vs' = insert ?v (vs\<^sub>1 \<union> vs\<^sub>2) \<and> 
+    \<kappa> = \<kappa>\<^sub>1 @ \<kappa>\<^sub>2 @ [(Var ?v, \<tau>\<^sub>1)]" by (simp add: Let_def)
+  from Let\<^sub>s have V: "?v \<noteq> y" by auto
+  thus ?case 
   proof (cases "x = z")
-    case True  
-  
-    from Let\<^sub>s have "typecheck' (\<Gamma>(x \<mapsto> Var y)) vs (Let\<^sub>s z e\<^sub>s\<^sub>1 e\<^sub>s\<^sub>2) = (e\<^sub>u, \<tau>, vs', \<kappa>)" by blast
-    with T1 T2 have E: "e\<^sub>u = Let\<^sub>s z e\<^sub>u\<^sub>1 e\<^sub>u\<^sub>2 \<and> \<tau>\<^sub>2 = \<tau> \<and> vs' = vs\<^sub>1 \<union> vs\<^sub>2 \<and> \<kappa> = \<kappa>\<^sub>1 @ \<kappa>\<^sub>2" by simp
-  
-  
-  
-    from Let\<^sub>s have "y \<in> vs" by simp
+    case True
     from Let\<^sub>s have "subst_vars \<Gamma> \<subseteq> vs - {y}" by simp
-    from Let\<^sub>s have "uvars \<tau>' \<subseteq> vs - {y}" by simp
-    from Let\<^sub>s have "finite vs" by simp
-  
-  
-  
-    have "(case typecheck' (\<Gamma>(x \<mapsto> \<tau>', z \<mapsto> subst [y \<mapsto> \<tau>'] \<tau>\<^sub>1)) (vs \<union> vs\<^sub>1) e\<^sub>s\<^sub>2 of
-       (e\<^sub>u\<^sub>2, \<tau>\<^sub>2, vs\<^sub>2, \<kappa>\<^sub>2) \<Rightarrow>
-         (Let\<^sub>s z (map_expr\<^sub>s (subst [y \<mapsto> \<tau>']) e\<^sub>u\<^sub>1) e\<^sub>u\<^sub>2, \<tau>\<^sub>2, vs\<^sub>1 \<union> vs\<^sub>2,
-          constr_subst y \<tau>' \<kappa>\<^sub>1 @ \<kappa>\<^sub>2)) =
-      (Let\<^sub>s z (map_expr\<^sub>s (subst [y \<mapsto> \<tau>']) e\<^sub>u\<^sub>1) (map_expr\<^sub>s (subst [y \<mapsto> \<tau>']) e\<^sub>u\<^sub>2), subst [y \<mapsto> \<tau>'] \<tau>\<^sub>2,
-       vs\<^sub>1 \<union> vs\<^sub>2, constr_subst y \<tau>' \<kappa>\<^sub>1 @ constr_subst y \<tau>' \<kappa>\<^sub>2)" by (simp split: prod.splits)
-    with TC1 E have "typecheck' (\<Gamma>(x \<mapsto> \<tau>')) vs (Let\<^sub>s z e\<^sub>s\<^sub>1 e\<^sub>s\<^sub>2) =
-      (map_expr\<^sub>s (subst [y \<mapsto> \<tau>']) e\<^sub>u, subst [y \<mapsto> \<tau>'] \<tau>, vs', constr_subst y \<tau>' \<kappa>)" by simp
-    thus ?thesis by blast
+    with V have "y \<notin> subst_vars (\<Gamma>(z \<mapsto> Var ?v))" by (auto simp add: subst_vars_def ran_def)
+    with Let\<^sub>s T1 T2 True have "y \<notin> tyvars\<^sub>s e\<^sub>u\<^sub>2 \<and> y \<notin> uvars \<tau>\<^sub>2 \<and> y \<notin> constr_vars \<kappa>\<^sub>2" by simp
+    with V T1' T2 True have "typecheck' (\<Gamma>(x \<mapsto> \<tau>')) vs (Let\<^sub>s z e\<^sub>s\<^sub>1 e\<^sub>s\<^sub>2) =
+      (map_expr\<^sub>s (subst [y \<mapsto> \<tau>']) (Let\<^sub>s z e\<^sub>u\<^sub>1 e\<^sub>u\<^sub>2), subst [y \<mapsto> \<tau>'] \<tau>\<^sub>2, insert ?v (vs\<^sub>1 \<union> vs\<^sub>2), 
+        constr_subst y \<tau>' (\<kappa>\<^sub>1 @ \<kappa>\<^sub>2 @ [(Var ?v, \<tau>\<^sub>1)]))" by (simp add: Let_def)
+    with E show ?thesis by blast
   next
     case False
-    with T2 have X: "typecheck' (\<Gamma>(z \<mapsto> \<tau>\<^sub>1, x \<mapsto> Var y)) (vs \<union> vs\<^sub>1) e\<^sub>s\<^sub>2 = (e\<^sub>u\<^sub>2, \<tau>\<^sub>2, vs\<^sub>2, \<kappa>\<^sub>2)" 
-      by (simp add: fun_upd_twist)
-    from Let\<^sub>s have Y: "subst_vars (\<Gamma>(z \<mapsto> \<tau>\<^sub>1)) \<subseteq> (vs \<union> vs\<^sub>1) - {y}" by simp
-    from Let\<^sub>s T1 have "finite (vs \<union> vs\<^sub>1)" by simp
-    with Let\<^sub>s X Y have TC2: "typecheck' (\<Gamma>(z \<mapsto> \<tau>\<^sub>1, x \<mapsto> \<tau>')) (vs \<union> vs\<^sub>1) e\<^sub>s\<^sub>2 =
+    with T2 have X: "typecheck' (\<Gamma>(z \<mapsto> Var ?v, x \<mapsto> Var y)) (insert ?v (vs \<union> vs\<^sub>1)) e\<^sub>s\<^sub>2 = 
+      (e\<^sub>u\<^sub>2, \<tau>\<^sub>2, vs\<^sub>2, \<kappa>\<^sub>2)" by (simp add: fun_upd_twist)
+    from Let\<^sub>s have "subst_vars \<Gamma> \<subseteq> insert (fresh vs) (vs \<union> vs\<^sub>1) - {y}" by auto
+    with T1 V have Y: "subst_vars (\<Gamma>(z \<mapsto> Var ?v)) \<subseteq> insert ?v (vs \<union> vs\<^sub>1) - {y}" by simp
+    from Let\<^sub>s T1 have "finite (insert ?v (vs \<union> vs\<^sub>1))" by simp
+    with Let\<^sub>s X Y have "typecheck' (\<Gamma>(z \<mapsto> Var ?v, x \<mapsto> \<tau>')) (insert ?v (vs \<union> vs\<^sub>1)) e\<^sub>s\<^sub>2 =
       (map_expr\<^sub>s (subst [y \<mapsto> \<tau>']) e\<^sub>u\<^sub>2, subst [y \<mapsto> \<tau>'] \<tau>\<^sub>2, vs\<^sub>2, constr_subst y \<tau>' \<kappa>\<^sub>2)" by blast
-  
-  
-  
-    from Let\<^sub>s have "typecheck' (\<Gamma>(x \<mapsto> Var y)) vs (Let\<^sub>s z e\<^sub>s\<^sub>1 e\<^sub>s\<^sub>2) = (e\<^sub>u, \<tau>, vs', \<kappa>)" by blast
-    with T1 T2 have E: "e\<^sub>u = Let\<^sub>s z e\<^sub>u\<^sub>1 e\<^sub>u\<^sub>2 \<and> \<tau>\<^sub>2 = \<tau> \<and> vs' = vs\<^sub>1 \<union> vs\<^sub>2 \<and> \<kappa> = \<kappa>\<^sub>1 @ \<kappa>\<^sub>2" by simp
-  
-  
-  
-    from Let\<^sub>s have "y \<in> vs" by simp
-    from Let\<^sub>s have "subst_vars \<Gamma> \<subseteq> vs - {y}" by simp
-    from Let\<^sub>s have "uvars \<tau>' \<subseteq> vs - {y}" by simp
-    from Let\<^sub>s have "finite vs" by simp
-
-
-  
-  
-    have "(case typecheck' (\<Gamma>(x \<mapsto> \<tau>', z \<mapsto> subst [y \<mapsto> \<tau>'] \<tau>\<^sub>1)) (vs \<union> vs\<^sub>1) e\<^sub>s\<^sub>2 of
-       (e\<^sub>u\<^sub>2, \<tau>\<^sub>2, vs\<^sub>2, \<kappa>\<^sub>2) \<Rightarrow>
-         (Let\<^sub>s z (map_expr\<^sub>s (subst [y \<mapsto> \<tau>']) e\<^sub>u\<^sub>1) e\<^sub>u\<^sub>2, \<tau>\<^sub>2, vs\<^sub>1 \<union> vs\<^sub>2,
-          constr_subst y \<tau>' \<kappa>\<^sub>1 @ \<kappa>\<^sub>2)) =
-      (Let\<^sub>s z (map_expr\<^sub>s (subst [y \<mapsto> \<tau>']) e\<^sub>u\<^sub>1) (map_expr\<^sub>s (subst [y \<mapsto> \<tau>']) e\<^sub>u\<^sub>2), subst [y \<mapsto> \<tau>'] \<tau>\<^sub>2,
-       vs\<^sub>1 \<union> vs\<^sub>2, constr_subst y \<tau>' \<kappa>\<^sub>1 @ constr_subst y \<tau>' \<kappa>\<^sub>2)" by simp
-    with TC1 E have "typecheck' (\<Gamma>(x \<mapsto> \<tau>')) vs (Let\<^sub>s z e\<^sub>s\<^sub>1 e\<^sub>s\<^sub>2) =
-      (map_expr\<^sub>s (subst [y \<mapsto> \<tau>']) e\<^sub>u, subst [y \<mapsto> \<tau>'] \<tau>, vs', constr_subst y \<tau>' \<kappa>)" by simp
-    thus ?thesis by blast
+    with False have "typecheck' (\<Gamma>(x \<mapsto> \<tau>', z \<mapsto> Var ?v)) (insert ?v (vs \<union> vs\<^sub>1)) e\<^sub>s\<^sub>2 =
+      (map_expr\<^sub>s (subst [y \<mapsto> \<tau>']) e\<^sub>u\<^sub>2, subst [y \<mapsto> \<tau>'] \<tau>\<^sub>2, vs\<^sub>2, constr_subst y \<tau>' \<kappa>\<^sub>2)" 
+        by (simp add: fun_upd_twist)
+    with V T1' have "typecheck' (\<Gamma>(x \<mapsto> \<tau>')) vs (Let\<^sub>s z e\<^sub>s\<^sub>1 e\<^sub>s\<^sub>2) =
+      (map_expr\<^sub>s (subst [y \<mapsto> \<tau>']) (Let\<^sub>s z e\<^sub>u\<^sub>1 e\<^sub>u\<^sub>2), subst [y \<mapsto> \<tau>'] \<tau>\<^sub>2, insert ?v (vs\<^sub>1 \<union> vs\<^sub>2), 
+        constr_subst y \<tau>' (\<kappa>\<^sub>1 @ \<kappa>\<^sub>2 @ [(Var ?v, \<tau>\<^sub>1)]))" by (simp add: Let_def)
+    with E show ?thesis by blast
   qed
 qed auto
 
@@ -579,7 +562,66 @@ next
   with E A B C D F G show ?case by blast
 next
   case (tc\<^sub>t_let e\<^sub>1 t\<^sub>1 x e\<^sub>2 t\<^sub>2)
-  then show ?case by simp
+  let ?v = "fresh vs"
+  obtain e\<^sub>u\<^sub>1 \<tau>\<^sub>1 vs\<^sub>1 \<kappa>\<^sub>1 where TC1: "typecheck' \<Gamma> (insert ?v vs) (erase e\<^sub>1) = (e\<^sub>u\<^sub>1, \<tau>\<^sub>1, vs\<^sub>1, \<kappa>\<^sub>1)" 
+    by (metis prod_cases4)
+  obtain e\<^sub>u\<^sub>2 \<tau>\<^sub>2 vs\<^sub>2 \<kappa>\<^sub>2 where TC2: "typecheck' (\<Gamma>(x \<mapsto> Var ?v)) (insert ?v (vs \<union> vs\<^sub>1)) (erase e\<^sub>2) =
+    (e\<^sub>u\<^sub>2, \<tau>\<^sub>2, vs\<^sub>2, \<kappa>\<^sub>2)" by (metis prod_cases4)
+  with tc\<^sub>t_let TC1 have E: "e\<^sub>u = Let\<^sub>s x e\<^sub>u\<^sub>1 e\<^sub>u\<^sub>2 \<and> \<tau> = \<tau>\<^sub>2 \<and> vs' = insert ?v (vs\<^sub>1 \<union> vs\<^sub>2) \<and> 
+    \<kappa> = \<kappa>\<^sub>1 @ \<kappa>\<^sub>2 @ [(Var ?v, \<tau>\<^sub>1)]" by (simp add: Let_def)
+  from tc\<^sub>t_let have "subst_vars \<Gamma> \<subseteq> insert ?v vs" by auto
+  with tc\<^sub>t_let TC1 obtain \<sigma>\<^sub>1 where S1: "
+    map_expr\<^sub>s (eliminate_vars (insert ?v vs)) (map_expr\<^sub>s (subst \<sigma>\<^sub>1) e\<^sub>u\<^sub>1) = map_expr\<^sub>s to_unifiable e\<^sub>1 \<and>
+    eliminate_vars (insert ?v vs) (subst \<sigma>\<^sub>1 \<tau>\<^sub>1) = to_unifiable t\<^sub>1 \<and> dom \<sigma>\<^sub>1 = vs\<^sub>1 \<and>
+    subst_vars \<sigma>\<^sub>1 = {} \<and> \<sigma>\<^sub>1 unifies\<^sub>\<kappa> eliminate_vars_constr (insert ?v vs) \<kappa>\<^sub>1 \<and> valid_ty_subst \<sigma>\<^sub>1 \<and> 
+    idempotent \<sigma>\<^sub>1" by blast
+  from tc\<^sub>t_let have X: "subst_vars \<Gamma> \<subseteq> insert ?v (vs \<union> vs\<^sub>1) - {?v}" by auto
+  from tc\<^sub>t_let TC1 have U: "uvars \<tau>\<^sub>1 \<subseteq> vs\<^sub>1 \<union> subst_vars \<Gamma>" by simp
+  have "uvars (subst \<sigma>\<^sub>1 \<tau>\<^sub>1) \<subseteq> uvars \<tau>\<^sub>1 - dom \<sigma>\<^sub>1 \<union> subst_vars \<sigma>\<^sub>1" by simp
+  with S1 U have U': "uvars (subst \<sigma>\<^sub>1 \<tau>\<^sub>1) \<subseteq> subst_vars \<Gamma>" by blast
+  with tc\<^sub>t_let have Y: "uvars (subst \<sigma>\<^sub>1 \<tau>\<^sub>1) \<subseteq> insert ?v (vs \<union> vs\<^sub>1) - {?v}" by auto
+  from tc\<^sub>t_let TC1 have "finite (insert ?v (vs \<union> vs\<^sub>1))" by simp
+  with TC2 X Y have TC2': "typecheck' (\<Gamma>(x \<mapsto> subst \<sigma>\<^sub>1 \<tau>\<^sub>1)) (insert ?v (vs \<union> vs\<^sub>1)) (erase e\<^sub>2) = 
+    (map_expr\<^sub>s (subst [?v \<mapsto> subst \<sigma>\<^sub>1 \<tau>\<^sub>1]) e\<^sub>u\<^sub>2, subst [?v \<mapsto> subst \<sigma>\<^sub>1 \<tau>\<^sub>1] \<tau>\<^sub>2, vs\<^sub>2, 
+      constr_subst ?v (subst \<sigma>\<^sub>1 \<tau>\<^sub>1) \<kappa>\<^sub>2)" by simp
+
+  from S1 have T1: "t\<^sub>1 = to_type (eliminate_vars (insert ?v vs) (subst \<sigma>\<^sub>1 \<tau>\<^sub>1))" by simp
+  from tc\<^sub>t_let U' have "uvars (subst \<sigma>\<^sub>1 \<tau>\<^sub>1) \<subseteq> insert ?v vs" by auto
+  with T1 have A: "(map_option to_type \<circ> \<Gamma>)(x \<mapsto> t\<^sub>1) = map_option to_type \<circ> (\<Gamma>(x \<mapsto> subst \<sigma>\<^sub>1 \<tau>\<^sub>1))" 
+    by simp
+  from X Y have B: "subst_vars (\<Gamma>(x \<mapsto> subst \<sigma>\<^sub>1 \<tau>\<^sub>1)) \<subseteq> insert ?v (vs \<union> vs\<^sub>1)" 
+    by (auto simp add: subst_vars_def ran_def)
+  from tc\<^sub>t_let TC1 have "valid_ty_term \<tau>\<^sub>1" by auto
+  with S1 have "valid_ty_term (subst \<sigma>\<^sub>1 \<tau>\<^sub>1)" by simp
+  with tc\<^sub>t_let have C: "valid_ty_subst (\<Gamma>(x \<mapsto> subst \<sigma>\<^sub>1 \<tau>\<^sub>1))" by simp
+  from tc\<^sub>t_let TC1 have "finite (insert ?v (vs \<union> vs\<^sub>1))" by simp
+  with tc\<^sub>t_let TC2' A B C obtain \<sigma>\<^sub>2 where S2: "map_expr\<^sub>s (eliminate_vars (insert ?v (vs \<union> vs\<^sub>1))) 
+    (map_expr\<^sub>s (subst \<sigma>\<^sub>2) (map_expr\<^sub>s (subst [?v \<mapsto> subst \<sigma>\<^sub>1 \<tau>\<^sub>1]) e\<^sub>u\<^sub>2)) = map_expr\<^sub>s to_unifiable e\<^sub>2 \<and>
+    eliminate_vars (insert ?v (vs \<union> vs\<^sub>1)) (subst \<sigma>\<^sub>2 (subst [?v \<mapsto> subst \<sigma>\<^sub>1 \<tau>\<^sub>1] \<tau>\<^sub>2)) = to_unifiable t\<^sub>2 \<and>
+    dom \<sigma>\<^sub>2 = vs\<^sub>2 \<and> subst_vars \<sigma>\<^sub>2 = {} \<and> 
+    \<sigma>\<^sub>2 unifies\<^sub>\<kappa> eliminate_vars_constr (insert ?v (vs \<union> vs\<^sub>1)) (constr_subst ?v (subst \<sigma>\<^sub>1 \<tau>\<^sub>1) \<kappa>\<^sub>2) \<and> 
+    valid_ty_subst \<sigma>\<^sub>2 \<and> idempotent \<sigma>\<^sub>2" by presburger
+
+
+  from tc\<^sub>t_let have "map_option to_type \<circ> \<Gamma> \<turnstile>\<^sub>t e\<^sub>1 : t\<^sub>1" by simp
+  from tc\<^sub>t_let have "(map_option to_type \<circ> \<Gamma>)(x \<mapsto> t\<^sub>1) \<turnstile>\<^sub>t e\<^sub>2 : t\<^sub>2" by simp
+  from tc\<^sub>t_let have "finite vs" by simp
+  from tc\<^sub>t_let have "subst_vars \<Gamma> \<subseteq> vs" by simp
+  from tc\<^sub>t_let have "valid_ty_subst \<Gamma>" by simp
+
+  let ?\<sigma> = "extend_subst ?v (to_unifiable t\<^sub>2) (combine_subst \<sigma>\<^sub>1 \<sigma>\<^sub>2)"
+
+  from tc\<^sub>t_let TC1 have "insert ?v vs \<inter> vs\<^sub>1 = {}" by simp
+  hence V1: "?v \<notin> vs\<^sub>1" by simp
+
+
+
+  have "map_expr\<^sub>s (eliminate_vars vs) (map_expr\<^sub>s (subst ?\<sigma>) (Let\<^sub>s x e\<^sub>u\<^sub>1 e\<^sub>u\<^sub>2)) = 
+    map_expr\<^sub>s to_unifiable (Let\<^sub>s x e\<^sub>1 e\<^sub>2) \<and> eliminate_vars vs (subst ?\<sigma> \<tau>\<^sub>2) = to_unifiable t\<^sub>2 \<and> 
+    dom ?\<sigma> = insert ?v (vs\<^sub>1 \<union> vs\<^sub>2) \<and> subst_vars ?\<sigma> = {} \<and> 
+    ?\<sigma> unifies\<^sub>\<kappa> eliminate_vars_constr vs (\<kappa>\<^sub>1 @ \<kappa>\<^sub>2 @ [(Var ?v, \<tau>\<^sub>1)]) \<and> 
+    valid_ty_subst ?\<sigma> \<and> idempotent ?\<sigma>" by simp
+  with E show ?case by blast
 qed auto
 
 text \<open>With \<open>typecheck_finds_subst\<close> in hand, our failure case is now quite simple:\<close>
