09ChainedEnvironment/ChainedEnvironment.thy
@@ -57,7 +57,7 @@ inductive eval\<^sub>v :: "code\<^sub>b list \<Rightarrow> state\<^sub>v \<Right
     halloc \<Delta> (v\<^sub>1, p\<^sub>\<Delta>') = (\<Delta>', p\<^sub>\<Delta>'') \<Longrightarrow> 
       \<C> \<tturnstile> S\<^sub>v h \<Delta> (v\<^sub>1 # v\<^sub>2 # \<V>) ((p\<^sub>\<Delta>, Suc p\<^sub>\<C>) # s) \<leadsto>\<^sub>v S\<^sub>v h \<Delta>' \<V> ((Suc p\<^sub>\<Delta>'', p\<^sub>\<C>') # (p\<^sub>\<Delta>, p\<^sub>\<C>) # s)"
 | ev\<^sub>v_pushenv [simp]: "lookup \<C> p\<^sub>\<C> = Some PushEnv\<^sub>b \<Longrightarrow> halloc \<Delta> (v, p\<^sub>\<Delta>) = (\<Delta>', p\<^sub>\<Delta>') \<Longrightarrow> 
-    \<C> \<tturnstile> S\<^sub>v h \<Delta> (v # \<V>) ((p\<^sub>\<Delta>, Suc p\<^sub>\<C>) # s) \<leadsto>\<^sub>v S\<^sub>v h \<Delta>' \<V> ((p\<^sub>\<Delta>', p\<^sub>\<C>) # s)"
+    \<C> \<tturnstile> S\<^sub>v h \<Delta> (v # \<V>) ((p\<^sub>\<Delta>, Suc p\<^sub>\<C>) # s) \<leadsto>\<^sub>v S\<^sub>v h \<Delta>' \<V> ((Suc p\<^sub>\<Delta>', p\<^sub>\<C>) # s)"
 | ev\<^sub>v_return [simp]: "lookup \<C> p\<^sub>\<C> = Some Return\<^sub>b \<Longrightarrow> 
     \<C> \<tturnstile> S\<^sub>v h \<Delta> \<V> ((p\<^sub>\<Delta>, Suc p\<^sub>\<C>) # s) \<leadsto>\<^sub>v S\<^sub>v h \<Delta> \<V> s"
 | ev\<^sub>v_jump [simp]: "lookup \<C> p\<^sub>\<C> = Some Jump\<^sub>b \<Longrightarrow> hlookup h v\<^sub>2 = Lam\<^sub>v p\<^sub>\<Delta>' p\<^sub>\<C>' \<Longrightarrow>
